src/CFG/Collecting/CFG_Compound_Paths.thy
@@ -110,18 +110,17 @@ qed
 
 lemma cfg_path_mono_edges[intro]:
   assumes sub: "edges g \<subseteq> edges h"
-    and p: "cfg_path g u es v"
-  shows "cfg_path h u es v"
+    and p: "g \<turnstile> u \<longrightarrow>\<^bsub>es\<^esub> v"
+  shows "h \<turnstile> u \<longrightarrow>\<^bsub>es\<^esub> v"
   using p sub by (induction rule: cfg_path.induct) (auto intro: cfg_path.intros subsetD)
 
 lemma cfg_path_sub_offset_into:
   assumes c0: "compile c 0 = (n, en, ex, E)"
-    and p: "cfg_path (to_cfg c) en es ex"
+    and p: "(to_cfg c) \<turnstile> en \<longrightarrow>\<^bsub>es\<^esub> ex"
     and sub: "edges (mk_cfg (en + k) (ex + k) (offset_edges k E)) \<subseteq> edges g"
-  shows "cfg_path g (en + k) (offset_path k es) (ex + k)"
+  shows "g \<turnstile> (en + k) \<longrightarrow>\<^bsub>(offset_path k es)\<^esub> (ex + k)"
 proof -
-  have p_off: "cfg_path (mk_cfg (en + k) (ex + k) (offset_edges k E))
-                      (en + k) (offset_path k es) (ex + k)"
+  have p_off: "(mk_cfg (en + k) (ex + k) (offset_edges k E)) \<turnstile> (en + k) \<longrightarrow>\<^bsub>(offset_path k es)\<^esub> (ex + k)"
     using cfg_path_offset[OF p[unfolded to_cfg_mk[OF c0]]] .
   show ?thesis by (rule cfg_path_mono_edges[OF sub p_off])
 qed
@@ -200,22 +199,22 @@ qed
 lemma cfg_path_Seq_in_c2:
   assumes c1: "compile c1 0 = (n1, en1, ex1, E1)"
     and c2_0: "compile c2 0 = (n20, en20, ex20, E20)"
-    and p: "cfg_path (to_cfg (c1 ;; c2)) u es v"
+    and p: "(to_cfg (c1 ;; c2)) \<turnstile> u \<longrightarrow>\<^bsub>es\<^esub> v"
     and u_ge: "n1 \<le> u"
   shows "\<exists>es'. es = offset_path n1 es' \<and>
-                cfg_path (to_cfg c2) (u - n1) es' (v - n1)"
+                (to_cfg c2) \<turnstile> (u - n1) \<longrightarrow>\<^bsub>es'\<^esub> (v - n1)"
   using p u_ge
 proof (induction es arbitrary: u)
   case Nil
   from Nil(1) have "u = v" by (cases rule: cfg_path.cases) simp_all
-  hence "cfg_path (to_cfg c2) (u - n1) [] (v - n1)" by (simp add: cfg_path.empty)
+  hence "(to_cfg c2) \<turnstile> (u - n1) \<longrightarrow>\<^bsub>[]\<^esub> (v - n1)" by (simp add: cfg_path.empty)
   thus ?case by (rule_tac x = "[]" in exI) simp
 next
   case (Cons hd tl)
   obtain a w where hd_eq: "hd = (a, w)" by (cases hd) auto
   from Cons.prems(1) hd_eq obtain
         e_compound: "(u, a, w) \<in> edges (to_cfg (c1 ;; c2))"
-    and ps: "cfg_path (to_cfg (c1 ;; c2)) w tl v"
+    and ps: "(to_cfg (c1 ;; c2)) \<turnstile> w \<longrightarrow>\<^bsub>tl\<^esub> v"
     by (cases rule: cfg_path.cases) auto
   have e_off: "(u, a, w) \<in> offset_edges n1 E20"
     using compound_Seq_edge_src_ge_n1[OF c1 c2_0 e_compound Cons.prems(2)] .
@@ -225,14 +224,14 @@ next
   have kw: "n1 \<le> w" using decomp(2) by simp
   from Cons.IH[OF ps kw] obtain es' where
         es_eq: "tl = offset_path n1 es'"
-    and pe2: "cfg_path (to_cfg c2) (w - n1) es' (v - n1)"
+    and pe2: "(to_cfg c2) \<turnstile> (w - n1) \<longrightarrow>\<^bsub>es'\<^esub> (v - n1)"
     by auto
   have toc2_edges: "edges (to_cfg c2) = E20"
     using c2_0 by (simp add: to_cfg_simps)
   have edge_c2: "(u - n1, a, w - n1) \<in> edges (to_cfg c2)"
     using toc2_edges decomp by simp
   let ?es'_full = "(a, w - n1) # es'"
-  have p_full: "cfg_path (to_cfg c2) (u - n1) ?es'_full (v - n1)"
+  have p_full: "(to_cfg c2) \<turnstile> (u - n1) \<longrightarrow>\<^bsub>?es'_full\<^esub> (v - n1)"
     by (rule cfg_path.step[OF edge_c2 pe2])
   have list_eq: "(a, w) # tl = offset_path n1 ?es'_full"
     using es_eq decomp(2) by simp
@@ -250,12 +249,12 @@ qed
 lemma cfg_path_Seq_split:
   assumes c1: "compile c1 0 = (n1, en1, ex1, E1)"
     and c2_0: "compile c2 0 = (n20, en20, ex20, E20)"
-    and p: "cfg_path (to_cfg (c1 ;; c2)) u es (ex20 + n1)"
+    and p: "(to_cfg (c1 ;; c2)) \<turnstile> u \<longrightarrow>\<^bsub>es\<^esub> (ex20 + n1)"
     and u_lt: "u < n1"
   shows "\<exists>es1 es2.
            es = es1 @ (EA_Nop, en20 + n1) # offset_path n1 es2 \<and>
-           cfg_path (to_cfg c1) u es1 ex1 \<and>
-           cfg_path (to_cfg c2) en20 es2 ex20"
+           (to_cfg c1) \<turnstile> u \<longrightarrow>\<^bsub>es1\<^esub> ex1 \<and>
+           (to_cfg c2) \<turnstile> en20 \<longrightarrow>\<^bsub>es2\<^esub> ex20"
   using p u_lt
 proof (induction es arbitrary: u)
   case Nil
@@ -266,7 +265,7 @@ next
   obtain a w where hd_eq: "hd = (a, w)" by (cases hd) auto
   from Cons.prems(1) hd_eq obtain
         e_compound: "(u, a, w) \<in> edges (to_cfg (c1 ;; c2))"
-    and ps: "cfg_path (to_cfg (c1 ;; c2)) w tl (ex20 + n1)"
+    and ps: "(to_cfg (c1 ;; c2)) \<turnstile> w \<longrightarrow>\<^bsub>tl\<^esub> (ex20 + n1)"
     by (cases rule: cfg_path.cases) auto
   from compound_Seq_edge_src_lt_n1[OF c1 c2_0 e_compound Cons.prems(2)]
   consider (E1) "(u, a, w) \<in> E1" | (bridge) "u = ex1" "a = EA_Nop" "w = en20 + n1"
@@ -277,14 +276,14 @@ next
     from compile_fresh[OF c1] E1 have w_lt: "w < n1" by auto
     from Cons.IH[OF ps w_lt] obtain es1 es2 where
           tl_eq: "tl = es1 @ (EA_Nop, en20 + n1) # offset_path n1 es2"
-      and p1: "cfg_path (to_cfg c1) w es1 ex1"
-      and p2: "cfg_path (to_cfg c2) en20 es2 ex20"
+      and p1: "(to_cfg c1) \<turnstile> w \<longrightarrow>\<^bsub>es1\<^esub> ex1"
+      and p2: "(to_cfg c2) \<turnstile> en20 \<longrightarrow>\<^bsub>es2\<^esub> ex20"
       by blast
     have toc1_edges: "edges (to_cfg c1) = E1"
       using c1 by (simp add: to_cfg_simps)
     have edge_c1: "(u, a, w) \<in> edges (to_cfg c1)" using E1 toc1_edges by simp
     let ?es1_full = "(a, w) # es1"
-    have p1_full: "cfg_path (to_cfg c1) u ?es1_full ex1"
+    have p1_full: "(to_cfg c1) \<turnstile> u \<longrightarrow>\<^bsub>?es1_full\<^esub> ex1"
       by (rule cfg_path.step[OF edge_c1 p1])
     have list_eq: "(a, w) # tl = ?es1_full @ (EA_Nop, en20 + n1) # offset_path n1 es2"
       using tl_eq by simp
@@ -295,12 +294,12 @@ next
     have w_ge: "n1 \<le> w" using bridge(3) by simp
     from cfg_path_Seq_in_c2[OF c1 c2_0 ps w_ge] obtain es' where
           tl_eq: "tl = offset_path n1 es'"
-      and pe2: "cfg_path (to_cfg c2) (w - n1) es' ((ex20 + n1) - n1)"
+      and pe2: "(to_cfg c2) \<turnstile> (w - n1) \<longrightarrow>\<^bsub>es'\<^esub> ((ex20 + n1) - n1)"
       by auto
     have wn: "w - n1 = en20" using bridge(3) by simp
     have exn: "(ex20 + n1) - n1 = ex20" by simp
-    have p2: "cfg_path (to_cfg c2) en20 es' ex20" using pe2 wn exn by simp
-    have p1: "cfg_path (to_cfg c1) u [] ex1"
+    have p2: "(to_cfg c2) \<turnstile> en20 \<longrightarrow>\<^bsub>es'\<^esub> ex20" using pe2 wn exn by simp
+    have p1: "(to_cfg c1) \<turnstile> u \<longrightarrow>\<^bsub>[]\<^esub> ex1"
       using bridge(1) by (simp add: cfg_path.empty)
     have list_eq: "(a, w) # tl = [] @ (EA_Nop, en20 + n1) # offset_path n1 es'"
       using bridge tl_eq by simp
@@ -313,28 +312,28 @@ qed
 lemma cfg_path_Seq_iff:
   assumes c1: "compile c1 0 = (n1, en1, ex1, E1)"
     and c2_0: "compile c2 0 = (n20, en20, ex20, E20)"
-  shows "cfg_path (to_cfg (c1 ;; c2)) en1 es (ex20 + n1)
+  shows "(to_cfg (c1 ;; c2)) \<turnstile> en1 \<longrightarrow>\<^bsub>es\<^esub> (ex20 + n1)
          \<longleftrightarrow> (\<exists>es1 es2.
               es = es1 @ (EA_Nop, en20 + n1) # offset_path n1 es2
-              \<and> cfg_path (to_cfg c1) en1 es1 ex1
-              \<and> cfg_path (to_cfg c2) en20 es2 ex20)"
+              \<and> (to_cfg c1) \<turnstile> en1 \<longrightarrow>\<^bsub>es1\<^esub> ex1
+              \<and> (to_cfg c2) \<turnstile> en20 \<longrightarrow>\<^bsub>es2\<^esub> ex20)"
 proof (intro iffI)
-  assume p: "cfg_path (to_cfg (c1 ;; c2)) en1 es (ex20 + n1)"
+  assume p: "(to_cfg (c1 ;; c2)) \<turnstile> en1 \<longrightarrow>\<^bsub>es\<^esub> (ex20 + n1)"
   show "\<exists>es1 es2.
           es = es1 @ (EA_Nop, en20 + n1) # offset_path n1 es2
-          \<and> cfg_path (to_cfg c1) en1 es1 ex1
-          \<and> cfg_path (to_cfg c2) en20 es2 ex20"
+          \<and> (to_cfg c1) \<turnstile> en1 \<longrightarrow>\<^bsub>es1\<^esub> ex1
+          \<and> (to_cfg c2) \<turnstile> en20 \<longrightarrow>\<^bsub>es2\<^esub> ex20"
     using cfg_path_Seq_split[OF c1 c2_0 p] compile_fresh[OF c1]
     by auto
 next
   assume "\<exists>es1 es2.
           es = es1 @ (EA_Nop, en20 + n1) # offset_path n1 es2
-          \<and> cfg_path (to_cfg c1) en1 es1 ex1
-          \<and> cfg_path (to_cfg c2) en20 es2 ex20"
+          \<and> (to_cfg c1) \<turnstile> en1 \<longrightarrow>\<^bsub>es1\<^esub> ex1
+          \<and> (to_cfg c2) \<turnstile> en20 \<longrightarrow>\<^bsub>es2\<^esub> ex20"
   then obtain es1 es2 where
         es_eq: "es = es1 @ (EA_Nop, en20 + n1) # offset_path n1 es2"
-    and p1: "cfg_path (to_cfg c1) en1 es1 ex1"
-    and p2: "cfg_path (to_cfg c2) en20 es2 ex20"
+    and p1: "(to_cfg c1) \<turnstile> en1 \<longrightarrow>\<^bsub>es1\<^esub> ex1"
+    and p2: "(to_cfg c2) \<turnstile> en20 \<longrightarrow>\<^bsub>es2\<^esub> ex20"
     by blast
     have c2_n: "compile c2 n1 =
                 (n20 + n1, en20 + n1, ex20 + n1, offset_edges n1 E20)"
@@ -344,16 +343,16 @@ next
       using cfg_edges_entry_exit_Seq[OF c1 c2_n] by auto
     have sub_c1: "edges (to_cfg c1) \<subseteq> edges (to_cfg (c1 ;; c2))"
       unfolding to_cfg_mk[OF c1] using Eseq by auto
-    have es1_in: "cfg_path (to_cfg (c1 ;; c2)) en1 es1 ex1"
+    have es1_in: "(to_cfg (c1 ;; c2)) \<turnstile> en1 \<longrightarrow>\<^bsub>es1\<^esub> ex1"
       by (rule cfg_path_mono_edges[OF sub_c1 p1])
-    have bridge: "cfg_path (to_cfg (c1 ;; c2)) ex1 [(EA_Nop, en20 + n1)] (en20 + n1)"
+    have bridge: "(to_cfg (c1 ;; c2)) \<turnstile> ex1 \<longrightarrow>\<^bsub>[(EA_Nop, en20 + n1)]\<^esub> (en20 + n1)"
       using Eseq by (auto intro: cfg_path.intros)
     have sub_off: "edges (mk_cfg (en20 + n1) (ex20 + n1) (offset_edges n1 E20))
                     \<subseteq> edges (to_cfg (c1 ;; c2))"
       using Eseq by auto
-    have es2_in: "cfg_path (to_cfg (c1 ;; c2)) (en20 + n1) (offset_path n1 es2) (ex20 + n1)"
+    have es2_in: "(to_cfg (c1 ;; c2)) \<turnstile> (en20 + n1) \<longrightarrow>\<^bsub>(offset_path n1 es2)\<^esub> (ex20 + n1)"
       by (rule cfg_path_sub_offset_into[OF c2_0 p2 sub_off])
-    show "cfg_path (to_cfg (c1 ;; c2)) en1 es (ex20 + n1)"
+    show "(to_cfg (c1 ;; c2)) \<turnstile> en1 \<longrightarrow>\<^bsub>es\<^esub> (ex20 + n1)"
       using cfg_path_append[OF cfg_path_append[OF es1_in bridge] es2_in] es_eq by simp
 qed
 
@@ -456,10 +455,10 @@ qed
 lemma cfg_path_If_factor_c1:
   assumes c1: "compile c1 0 = (n10, en10, ex10, E10)"
     and c2: "compile c2 0 = (n20, en20, ex20, E20)"
-    and p: "cfg_path (to_cfg (IF b THEN c1 ELSE c2)) u es (n20 + (n10 + 1))"
+    and p: "(to_cfg (IF b THEN c1 ELSE c2)) \<turnstile> u \<longrightarrow>\<^bsub>es\<^esub> (n20 + (n10 + 1))"
     and u_in: "1 \<le> u" and u_lt: "u < n10 + 1"
   shows "\<exists>es'. es = offset_path 1 es' @ [(EA_Nop, n20 + (n10 + 1))] \<and>
-                cfg_path (to_cfg c1) (u - 1) es' ex10"
+                (to_cfg c1) \<turnstile> (u - 1) \<longrightarrow>\<^bsub>es'\<^esub> ex10"
   using p u_in u_lt
 proof (induction es arbitrary: u)
   case Nil
@@ -470,7 +469,7 @@ next
   obtain a w where hd_eq: "hd = (a, w)" by (cases hd) auto
   from Cons.prems(1) hd_eq obtain
         e_compound: "(u, a, w) \<in> edges (to_cfg (IF b THEN c1 ELSE c2))"
-    and ps: "cfg_path (to_cfg (IF b THEN c1 ELSE c2)) w tl (n20 + (n10 + 1))"
+    and ps: "(to_cfg (IF b THEN c1 ELSE c2)) \<turnstile> w \<longrightarrow>\<^bsub>tl\<^esub> (n20 + (n10 + 1))"
     by (cases rule: cfg_path.cases) auto
   from compound_If_edge_src_c1[OF c1 c2 e_compound Cons.prems(2) Cons.prems(3)]
   consider (E1) "(u, a, w) \<in> offset_edges 1 E10"
@@ -486,14 +485,14 @@ next
       using compile_fresh[OF c1] decomp(2,3) by force
     from Cons.IH[OF ps w_in w_lt] obtain es' where
           tl_eq: "tl = offset_path 1 es' @ [(EA_Nop, n20 + (n10 + 1))]"
-      and pe1: "cfg_path (to_cfg c1) (w - 1) es' ex10"
+      and pe1: "(to_cfg c1) \<turnstile> (w - 1) \<longrightarrow>\<^bsub>es'\<^esub> ex10"
       by auto
     have toc1_edges: "edges (to_cfg c1) = E10"
       using c1 by (simp add: to_cfg_simps)
     have edge_c1: "(u - 1, a, w - 1) \<in> edges (to_cfg c1)"
       using toc1_edges decomp by simp
     let ?es'_full = "(a, w - 1) # es'"
-    have p_full: "cfg_path (to_cfg c1) (u - 1) ?es'_full ex10"
+    have p_full: "(to_cfg c1) \<turnstile> (u - 1) \<longrightarrow>\<^bsub>?es'_full\<^esub> ex10"
       by (rule cfg_path.step[OF edge_c1 pe1])
     have list_eq: "(a, w) # tl = offset_path 1 ?es'_full @ [(EA_Nop, n20 + (n10 + 1))]"
       using tl_eq decomp(2) by simp
@@ -511,7 +510,7 @@ next
         by (cases rule: cfg_path.cases) auto
       from e_next w_n2 compound_If_no_source_n2[OF c1 c2] show False by blast
     qed
-    have empty_p: "cfg_path (to_cfg c1) (u - 1) [] ex10"
+    have empty_p: "(to_cfg c1) \<turnstile> (u - 1) \<longrightarrow>\<^bsub>[]\<^esub> ex10"
       using bridge(1) by (simp add: cfg_path.empty)
     have list_eq: "(a, w) # tl = offset_path 1 [] @ [(EA_Nop, n20 + (n10 + 1))]"
       using bridge tl_empty by simp
@@ -522,10 +521,10 @@ qed
 lemma cfg_path_If_factor_c2:
   assumes c1: "compile c1 0 = (n10, en10, ex10, E10)"
     and c2: "compile c2 0 = (n20, en20, ex20, E20)"
-    and p: "cfg_path (to_cfg (IF b THEN c1 ELSE c2)) u es (n20 + (n10 + 1))"
+    and p: "(to_cfg (IF b THEN c1 ELSE c2)) \<turnstile> u \<longrightarrow>\<^bsub>es\<^esub> (n20 + (n10 + 1))"
     and u_in: "n10 + 1 \<le> u" and u_lt: "u < n20 + (n10 + 1)"
   shows "\<exists>es'. es = offset_path (n10 + 1) es' @ [(EA_Nop, n20 + (n10 + 1))] \<and>
-                cfg_path (to_cfg c2) (u - (n10 + 1)) es' ex20"
+                (to_cfg c2) \<turnstile> (u - (n10 + 1)) \<longrightarrow>\<^bsub>es'\<^esub> ex20"
   using p u_in u_lt
 proof (induction es arbitrary: u)
   case Nil
@@ -536,7 +535,7 @@ next
   obtain a w where hd_eq: "hd = (a, w)" by (cases hd) auto
   from Cons.prems(1) hd_eq obtain
         e_compound: "(u, a, w) \<in> edges (to_cfg (IF b THEN c1 ELSE c2))"
-    and ps: "cfg_path (to_cfg (IF b THEN c1 ELSE c2)) w tl (n20 + (n10 + 1))"
+    and ps: "(to_cfg (IF b THEN c1 ELSE c2)) \<turnstile> w \<longrightarrow>\<^bsub>tl\<^esub> (n20 + (n10 + 1))"
     by (cases rule: cfg_path.cases) auto
   from compound_If_edge_src_c2[OF c1 c2 e_compound Cons.prems(2) Cons.prems(3)]
   consider (E2) "(u, a, w) \<in> offset_edges (n10 + 1) E20"
@@ -553,14 +552,14 @@ next
       using compile_fresh[OF c2] decomp(2,3) by force
     from Cons.IH[OF ps w_in w_lt] obtain es' where
           tl_eq: "tl = offset_path (n10 + 1) es' @ [(EA_Nop, n20 + (n10 + 1))]"
-      and pe2: "cfg_path (to_cfg c2) (w - (n10 + 1)) es' ex20"
+      and pe2: "(to_cfg c2) \<turnstile> (w - (n10 + 1)) \<longrightarrow>\<^bsub>es'\<^esub> ex20"
       by auto
     have toc2_edges: "edges (to_cfg c2) = E20"
       using c2 by (simp add: to_cfg_simps)
     have edge_c2: "(u - (n10 + 1), a, w - (n10 + 1)) \<in> edges (to_cfg c2)"
       using toc2_edges decomp by simp
     let ?es'_full = "(a, w - (n10 + 1)) # es'"
-    have p_full: "cfg_path (to_cfg c2) (u - (n10 + 1)) ?es'_full ex20"
+    have p_full: "(to_cfg c2) \<turnstile> (u - (n10 + 1)) \<longrightarrow>\<^bsub>?es'_full\<^esub> ex20"
       by (rule cfg_path.step[OF edge_c2 pe2])
     have list_eq: "(a, w) # tl = offset_path (n10 + 1) ?es'_full @ [(EA_Nop, n20 + (n10 + 1))]"
       using tl_eq decomp(2) by simp
@@ -578,7 +577,7 @@ next
         by (cases rule: cfg_path.cases) auto
       from e_next w_n2 compound_If_no_source_n2[OF c1 c2] show False by blast
     qed
-    have empty_p: "cfg_path (to_cfg c2) (u - (n10 + 1)) [] ex20"
+    have empty_p: "(to_cfg c2) \<turnstile> (u - (n10 + 1)) \<longrightarrow>\<^bsub>[]\<^esub> ex20"
       using bridge(1) by (simp add: cfg_path.empty)
     have list_eq: "(a, w) # tl = offset_path (n10 + 1) [] @ [(EA_Nop, n20 + (n10 + 1))]"
       using bridge tl_empty by simp
@@ -595,15 +594,15 @@ qed
 lemma cfg_path_If_split:
   assumes c1: "compile c1 0 = (n10, en10, ex10, E10)"
     and c2: "compile c2 0 = (n20, en20, ex20, E20)"
-    and p: "cfg_path (to_cfg (IF b THEN c1 ELSE c2)) 0 es (n20 + (n10 + 1))"
+    and p: "(to_cfg (IF b THEN c1 ELSE c2)) \<turnstile> 0 \<longrightarrow>\<^bsub>es\<^esub> (n20 + (n10 + 1))"
   shows "(\<exists>es1. es = (EA_Assume b, en10 + 1)
                      # offset_path 1 es1
                      @ [(EA_Nop, n20 + (n10 + 1))]
-              \<and> cfg_path (to_cfg c1) en10 es1 ex10)
+              \<and> (to_cfg c1) \<turnstile> en10 \<longrightarrow>\<^bsub>es1\<^esub> ex10)
        \<or> (\<exists>es2. es = (EA_AssumeNot b, en20 + (n10 + 1))
                      # offset_path (n10 + 1) es2
                      @ [(EA_Nop, n20 + (n10 + 1))]
-              \<and> cfg_path (to_cfg c2) en20 es2 ex20)"
+              \<and> (to_cfg c2) \<turnstile> en20 \<longrightarrow>\<^bsub>es2\<^esub> ex20)"
 proof -
   have c1_1: "compile c1 1 = (n10 + 1, en10 + 1, ex10 + 1, offset_edges 1 E10)"
     using compile_from_0_offsets[OF c1, of 1] by simp
@@ -629,7 +628,7 @@ proof -
   obtain a w where hd_eq: "hd = (a, w)" by (cases hd) auto
   from p es_cons hd_eq obtain
         e_first: "(0, a, w) \<in> edges (to_cfg (IF b THEN c1 ELSE c2))"
-    and ps: "cfg_path (to_cfg (IF b THEN c1 ELSE c2)) w tl (n20 + (n10 + 1))"
+    and ps: "(to_cfg (IF b THEN c1 ELSE c2)) \<turnstile> w \<longrightarrow>\<^bsub>tl\<^esub> (n20 + (n10 + 1))"
     by (cases rule: cfg_path.cases) auto
 
   from compile_fresh[OF c1] have ex10_lt: "ex10 < n10" by simp
@@ -658,10 +657,10 @@ proof -
     from compile_fresh[OF c1_1] have w_in: "1 \<le> w" "w < n10 + 1" using w_eq by auto
     from cfg_path_If_factor_c1[OF c1 c2 ps w_in(1) w_in(2)] obtain es1 where
           tl_eq: "tl = offset_path 1 es1 @ [(EA_Nop, n20 + (n10 + 1))]"
-      and pc1: "cfg_path (to_cfg c1) (w - 1) es1 ex10"
+      and pc1: "(to_cfg c1) \<turnstile> (w - 1) \<longrightarrow>\<^bsub>es1\<^esub> ex10"
       by blast
     have w_minus: "w - 1 = en10" using w_eq by simp
-    from pc1 w_minus have pc1': "cfg_path (to_cfg c1) en10 es1 ex10" by simp
+    from pc1 w_minus have pc1': "(to_cfg c1) \<turnstile> en10 \<longrightarrow>\<^bsub>es1\<^esub> ex10" by simp
     have es_eq:
       "es = (EA_Assume b, en10 + 1) # offset_path 1 es1 @ [(EA_Nop, n20 + (n10 + 1))]"
       using es_cons hd_eq a_eq w_eq tl_eq by simp
@@ -673,10 +672,10 @@ proof -
       have w_in: "n10 + 1 \<le> w" "w < n20 + (n10 + 1)" using w_eq by auto
     from cfg_path_If_factor_c2[OF c1 c2 ps w_in(1) w_in(2)] obtain es2 where
           tl_eq: "tl = offset_path (n10 + 1) es2 @ [(EA_Nop, n20 + (n10 + 1))]"
-      and pc2: "cfg_path (to_cfg c2) (w - (n10 + 1)) es2 ex20"
+      and pc2: "(to_cfg c2) \<turnstile> (w - (n10 + 1)) \<longrightarrow>\<^bsub>es2\<^esub> ex20"
       by blast
     have w_minus: "w - (n10 + 1) = en20" using w_eq by simp
-    from pc2 w_minus have pc2': "cfg_path (to_cfg c2) en20 es2 ex20" by simp
+    from pc2 w_minus have pc2': "(to_cfg c2) \<turnstile> en20 \<longrightarrow>\<^bsub>es2\<^esub> ex20" by simp
     have es_eq:
       "es = (EA_AssumeNot b, en20 + (n10 + 1)) # offset_path (n10 + 1) es2
              @ [(EA_Nop, n20 + (n10 + 1))]"
@@ -688,7 +687,7 @@ qed
 lemma cfg_path_singleton_edge:
   assumes E: "edges g = {(u0, a0, v0)}"
     and ne: "u0 \<noteq> v0"
-    and p: "cfg_path g u0 es v0"
+    and p: "g \<turnstile> u0 \<longrightarrow>\<^bsub>es\<^esub> v0"
   shows "es = [(a0, v0)]"
 proof (cases es)
   case Nil
@@ -698,7 +697,7 @@ next
   obtain a w where hd_eq: "hd = (a, w)" by (cases hd) auto
   from Cons hd_eq p obtain
         edge: "(u0, a, w) \<in> edges g"
-    and p_tl: "cfg_path g w tl v0"
+    and p_tl: "g \<turnstile> w \<longrightarrow>\<^bsub>tl\<^esub> v0"
     by (auto elim: cfg_path.cases)
   from edge E have aw: "a = a0" "w = v0" by auto
   have "tl = []"
@@ -788,14 +787,14 @@ qed
 lemma cfg_path_While_split_trailing_exit:
   assumes c0: "compile c 0 = (n10, en10, ex10, E10)"
     and c1: "compile c 1 = (n10 + 1, en10 + 1, ex10 + 1, offset_edges 1 E10)"
-    and p: "cfg_path (to_cfg (WHILE b DO c)) 0 es (n10 + 1)"
+    and p: "(to_cfg (WHILE b DO c)) \<turnstile> 0 \<longrightarrow>\<^bsub>es\<^esub> (n10 + 1)"
     and ne: "es \<noteq> []"
   shows "\<exists>es_pre. es = es_pre @ [(EA_AssumeNot b, n10 + 1)]
-          \<and> cfg_path (to_cfg (WHILE b DO c)) 0 es_pre 0"
+          \<and> (to_cfg (WHILE b DO c)) \<turnstile> 0 \<longrightarrow>\<^bsub>es_pre\<^esub> 0"
 proof -
   from cfg_path_split_last[OF p ne] obtain es_pre mid aa where
         spl: "es = es_pre @ [(aa, n10 + 1)]"
-    and p_pre: "cfg_path (to_cfg (WHILE b DO c)) 0 es_pre mid"
+    and p_pre: "(to_cfg (WHILE b DO c)) \<turnstile> 0 \<longrightarrow>\<^bsub>es_pre\<^esub> mid"
     and last_e: "(mid, aa, n10 + 1) \<in> edges (to_cfg (WHILE b DO c))"
     by blast
   from compound_While_edge_into_exit[OF c0 c1 last_e] have mid_aa: "mid = 0 \<and> aa = EA_AssumeNot b"
@@ -807,17 +806,17 @@ qed
 lemma cfg_path_While_loop_first_edge:
   assumes c0: "compile c 0 = (n10, en10, ex10, E10)"
     and c1: "compile c 1 = (n10 + 1, en10 + 1, ex10 + 1, offset_edges 1 E10)"
-    and p: "cfg_path (to_cfg (WHILE b DO c)) 0 es (0 :: pp)"
+    and p: "(to_cfg (WHILE b DO c)) \<turnstile> 0 \<longrightarrow>\<^bsub>es\<^esub> (0 :: pp)"
     and ne: "es \<noteq> []"
   obtains tl where "es = (EA_Assume b, en10 + 1) # tl"
-    and "cfg_path (to_cfg (WHILE b DO c)) (en10 + 1) tl 0"
+    and "(to_cfg (WHILE b DO c)) \<turnstile> (en10 + 1) \<longrightarrow>\<^bsub>tl\<^esub> 0"
 proof -
   obtain aa w tl where es_eq: "es = (aa, w) # tl"
     using ne p by auto
     
   from p es_eq obtain
         e0: "(0, aa, w) \<in> edges (to_cfg (WHILE b DO c))"
-    and ps: "cfg_path (to_cfg (WHILE b DO c)) w tl 0"
+    and ps: "(to_cfg (WHILE b DO c)) \<turnstile> w \<longrightarrow>\<^bsub>tl\<^esub> 0"
     by (cases rule: cfg_path.cases) auto
   have Ew: "edges (to_cfg (WHILE b DO c)) =
              {(0, EA_Assume b, en10 + 1), (0, EA_AssumeNot b, n10 + 1)}
@@ -826,8 +825,8 @@ proof -
   have not_assume_not: "\<not> (aa = EA_AssumeNot b \<and> w = n10 + 1)"
   proof
     assume H: "aa = EA_AssumeNot b \<and> w = n10 + 1"
-    with ps have "cfg_path (to_cfg (WHILE b DO c)) (n10 + 1) tl 0" by simp
-    moreover have "\<not> cfg_path (to_cfg (WHILE b DO c)) (n10 + 1) tl 0"
+    with ps have "(to_cfg (WHILE b DO c)) \<turnstile> (n10 + 1) \<longrightarrow>\<^bsub>tl\<^esub> 0" by simp
+    moreover have "\<not> (to_cfg (WHILE b DO c)) \<turnstile> (n10 + 1) \<longrightarrow>\<^bsub>tl\<^esub> 0"
     proof (cases tl)
       case Nil
       with calculation show ?thesis
@@ -853,11 +852,11 @@ lemma cfg_path_While_u_body_to_zero_split:
   assumes c0: "compile c 0 = (n10, en10, ex10, E10)"
     and c1: "compile c 1 = (n10 + 1, en10 + 1, ex10 + 1, offset_edges 1 E10)"
     and u_ge: "1 \<le> u" and u_lt: "u < n10 + 1"
-    and p: "cfg_path (to_cfg (WHILE b DO c)) u es (0 :: pp)"
+    and p: "(to_cfg (WHILE b DO c)) \<turnstile> u \<longrightarrow>\<^bsub>es\<^esub> (0 :: pp)"
   shows "\<exists>es_body es_rest.
       es = offset_path 1 es_body @ [(EA_Nop, 0)] @ es_rest
-      \<and> cfg_path (to_cfg c) (u - 1) es_body ex10
-      \<and> cfg_path (to_cfg (WHILE b DO c)) 0 es_rest 0"
+      \<and> (to_cfg c) \<turnstile> (u - 1) \<longrightarrow>\<^bsub>es_body\<^esub> ex10
+      \<and> (to_cfg (WHILE b DO c)) \<turnstile> 0 \<longrightarrow>\<^bsub>es_rest\<^esub> 0"
   using p u_ge u_lt
 proof (induction es arbitrary: u)
   case Nil
@@ -868,7 +867,7 @@ next
   obtain aa w where hd_eq: "hd = (aa, w)" by (cases hd) auto
   from Cons.prems(1) hd_eq obtain
         e_compound: "(u, aa, w) \<in> edges (to_cfg (WHILE b DO c))"
-    and ps: "cfg_path (to_cfg (WHILE b DO c)) w tl 0"
+    and ps: "(to_cfg (WHILE b DO c)) \<turnstile> w \<longrightarrow>\<^bsub>tl\<^esub> 0"
     by (cases rule: cfg_path.cases) auto
   from compound_While_edge_src_body[OF c0 c1 e_compound Cons.prems(2) Cons.prems(3)]
   consider (body) "(u, aa, w) \<in> offset_edges 1 E10"
@@ -890,15 +889,15 @@ next
       using decomp(2) by auto  
     from Cons.IH[OF ps w_ge w_lt] obtain es_body es_rest where
           tl_eq: "tl = offset_path 1 es_body @ [(EA_Nop, 0)] @ es_rest"
-      and pe1: "cfg_path (to_cfg c) (w - 1) es_body ex10"
-      and p0: "cfg_path (to_cfg (WHILE b DO c)) 0 es_rest 0"
+      and pe1: "(to_cfg c) \<turnstile> (w - 1) \<longrightarrow>\<^bsub>es_body\<^esub> ex10"
+      and p0: "(to_cfg (WHILE b DO c)) \<turnstile> 0 \<longrightarrow>\<^bsub>es_rest\<^esub> 0"
       by blast
     have toc_edges: "edges (to_cfg c) = E10"
       using c0 by (simp add: to_cfg_simps)
     have edge_c1: "(u - 1, aa, w - 1) \<in> edges (to_cfg c)"
       using toc_edges decomp by simp
     let ?esb = "(aa, w - 1) # es_body"
-    have p_body: "cfg_path (to_cfg c) (u - 1) ?esb ex10"
+    have p_body: "(to_cfg c) \<turnstile> (u - 1) \<longrightarrow>\<^bsub>?esb\<^esub> ex10"
       by (rule cfg_path.step[OF edge_c1 pe1])
     have list_eq: "(aa, w) # tl = offset_path 1 ?esb @ [(EA_Nop, 0)] @ es_rest"
       using tl_eq decomp(2) by simp
@@ -906,7 +905,7 @@ next
       using list_eq p_body p0 hd_eq by blast
   next
     case backa
-    have p_body: "cfg_path (to_cfg c) (u - 1) [] ex10"
+    have p_body: "(to_cfg c) \<turnstile> (u - 1) \<longrightarrow>\<^bsub>[]\<^esub> ex10"
       using backa(1) by (simp add: cfg_path.empty)
     have list_eq: "(aa, w) # tl = offset_path 1 [] @ [(EA_Nop, 0)] @ tl"
       using backa by simp
@@ -919,24 +918,24 @@ qed
 lemma cfg_path_While_loop_peel:
   assumes c0: "compile c 0 = (n10, en10, ex10, E10)"
     and c1: "compile c 1 = (n10 + 1, en10 + 1, ex10 + 1, offset_edges 1 E10)"
-    and p: "cfg_path (to_cfg (WHILE b DO c)) 0 es (0 :: pp)"
+    and p: "(to_cfg (WHILE b DO c)) \<turnstile> 0 \<longrightarrow>\<^bsub>es\<^esub> (0 :: pp)"
     and ne: "es \<noteq> []"
   shows "\<exists>es_body es_rest.
       es = [(EA_Assume b, en10 + 1)] @ offset_path 1 es_body @ [(EA_Nop, 0)] @ es_rest
-      \<and> cfg_path (to_cfg c) en10 es_body ex10
-      \<and> cfg_path (to_cfg (WHILE b DO c)) 0 es_rest 0"
+      \<and> (to_cfg c) \<turnstile> en10 \<longrightarrow>\<^bsub>es_body\<^esub> ex10
+      \<and> (to_cfg (WHILE b DO c)) \<turnstile> 0 \<longrightarrow>\<^bsub>es_rest\<^esub> 0"
 proof -
   from cfg_path_While_loop_first_edge[OF c0 c1 p ne] obtain tl where
         es_eq: "es = (EA_Assume b, en10 + 1) # tl"
-    and p_tl: "cfg_path (to_cfg (WHILE b DO c)) (en10 + 1) tl 0"
+    and p_tl: "(to_cfg (WHILE b DO c)) \<turnstile> (en10 + 1) \<longrightarrow>\<^bsub>tl\<^esub> 0"
     by blast
   from compile_fresh[OF c0] have en_lt: "en10 < n10" by simp
   hence u_ge: "1 \<le> en10 + 1" by simp
   have u_lt: "en10 + 1 < n10 + 1" using en_lt by simp
   from cfg_path_While_u_body_to_zero_split[OF c0 c1 u_ge u_lt p_tl] obtain es_body es_rest where
         tl_eq: "tl = offset_path 1 es_body @ [(EA_Nop, 0)] @ es_rest"
-    and pc: "cfg_path (to_cfg c) en10 es_body ex10"
-    and pr: "cfg_path (to_cfg (WHILE b DO c)) 0 es_rest 0"
+    and pc: "(to_cfg c) \<turnstile> en10 \<longrightarrow>\<^bsub>es_body\<^esub> ex10"
+    and pr: "(to_cfg (WHILE b DO c)) \<turnstile> 0 \<longrightarrow>\<^bsub>es_rest\<^esub> 0"
     by(auto)
   have es_full: "es = [(EA_Assume b, en10 + 1)] @ offset_path 1 es_body @ [(EA_Nop, 0)] @ es_rest"
     using es_eq tl_eq by simp
@@ -949,34 +948,34 @@ qed
 lemma cfg_path_If_iff:
   assumes c1: "compile c1 0 = (n10, en10, ex10, E10)"
     and c2: "compile c2 0 = (n20, en20, ex20, E20)"
-  shows "cfg_path (to_cfg (IF b THEN c1 ELSE c2)) 0 es (n20 + (n10 + 1))
+  shows "(to_cfg (IF b THEN c1 ELSE c2)) \<turnstile> 0 \<longrightarrow>\<^bsub>es\<^esub> (n20 + (n10 + 1))
          \<longleftrightarrow>
          ((\<exists>es1. es = (EA_Assume b, en10 + 1) # offset_path 1 es1
                         @ [(EA_Nop, n20 + (n10 + 1))]
-              \<and> cfg_path (to_cfg c1) en10 es1 ex10)
+              \<and> (to_cfg c1) \<turnstile> en10 \<longrightarrow>\<^bsub>es1\<^esub> ex10)
           \<or> (\<exists>es2. es = (EA_AssumeNot b, en20 + (n10 + 1))
                         # offset_path (n10 + 1) es2
                         @ [(EA_Nop, n20 + (n10 + 1))]
-              \<and> cfg_path (to_cfg c2) en20 es2 ex20))"
+              \<and> (to_cfg c2) \<turnstile> en20 \<longrightarrow>\<^bsub>es2\<^esub> ex20))"
 proof (intro iffI)
-  assume p: "cfg_path (to_cfg (IF b THEN c1 ELSE c2)) 0 es (n20 + (n10 + 1))"
+  assume p: "(to_cfg (IF b THEN c1 ELSE c2)) \<turnstile> 0 \<longrightarrow>\<^bsub>es\<^esub> (n20 + (n10 + 1))"
   show "((\<exists>es1. es = (EA_Assume b, en10 + 1) # offset_path 1 es1
                         @ [(EA_Nop, n20 + (n10 + 1))]
-              \<and> cfg_path (to_cfg c1) en10 es1 ex10)
+              \<and> (to_cfg c1) \<turnstile> en10 \<longrightarrow>\<^bsub>es1\<^esub> ex10)
           \<or> (\<exists>es2. es = (EA_AssumeNot b, en20 + (n10 + 1))
                         # offset_path (n10 + 1) es2
                         @ [(EA_Nop, n20 + (n10 + 1))]
-              \<and> cfg_path (to_cfg c2) en20 es2 ex20))"
+              \<and> (to_cfg c2) \<turnstile> en20 \<longrightarrow>\<^bsub>es2\<^esub> ex20))"
     using cfg_path_If_split[OF c1 c2 p] by blast
 next
   assume rhs: "((\<exists>es1. es = (EA_Assume b, en10 + 1) # offset_path 1 es1
                         @ [(EA_Nop, n20 + (n10 + 1))]
-              \<and> cfg_path (to_cfg c1) en10 es1 ex10)
+              \<and> (to_cfg c1) \<turnstile> en10 \<longrightarrow>\<^bsub>es1\<^esub> ex10)
           \<or> (\<exists>es2. es = (EA_AssumeNot b, en20 + (n10 + 1))
                         # offset_path (n10 + 1) es2
                         @ [(EA_Nop, n20 + (n10 + 1))]
-              \<and> cfg_path (to_cfg c2) en20 es2 ex20))"
-  show "cfg_path (to_cfg (IF b THEN c1 ELSE c2)) 0 es (n20 + (n10 + 1))"
+              \<and> (to_cfg c2) \<turnstile> en20 \<longrightarrow>\<^bsub>es2\<^esub> ex20))"
+  show "(to_cfg (IF b THEN c1 ELSE c2)) \<turnstile> 0 \<longrightarrow>\<^bsub>es\<^esub> (n20 + (n10 + 1))"
   proof -
     have c1_1: "compile c1 1 = (n10 + 1, en10 + 1, ex10 + 1, offset_edges 1 E10)"
       using compile_from_0_offsets[OF c1, of 1] by simp
@@ -994,37 +993,32 @@ next
     proof (elim disjE)
       assume left: "\<exists>es1. es = (EA_Assume b, en10 + 1) # offset_path 1 es1
                         @ [(EA_Nop, n20 + (n10 + 1))]
-                    \<and> cfg_path (to_cfg c1) en10 es1 ex10"
+                    \<and> (to_cfg c1) \<turnstile> en10 \<longrightarrow>\<^bsub>es1\<^esub> ex10"
       then obtain es1 where H: "es = (EA_Assume b, en10 + 1) # offset_path 1 es1
                         @ [(EA_Nop, n20 + (n10 + 1))]"
-        and p1: "cfg_path (to_cfg c1) en10 es1 ex10"
+        and p1: "(to_cfg c1) \<turnstile> en10 \<longrightarrow>\<^bsub>es1\<^esub> ex10"
         by blast
-      have es1_in: "cfg_path (to_cfg (IF b THEN c1 ELSE c2)) (en10 + 1)
-                                   (offset_path 1 es1) (ex10 + 1)"
+      have es1_in: "(to_cfg (IF b THEN c1 ELSE c2)) \<turnstile> (en10 + 1) \<longrightarrow>\<^bsub>(offset_path 1 es1)\<^esub> (ex10 + 1)"
         by (rule cfg_path_sub_offset_into[OF c1 p1]) (auto simp: Eif)
-      have head: "cfg_path (to_cfg (IF b THEN c1 ELSE c2)) 0 [(EA_Assume b, en10 + 1)] (en10 + 1)"
+      have head: "(to_cfg (IF b THEN c1 ELSE c2)) \<turnstile> 0 \<longrightarrow>\<^bsub>[(EA_Assume b, en10 + 1)]\<^esub> (en10 + 1)"
         using Eif by (auto intro: cfg_path.intros)
-      have tail: "cfg_path (to_cfg (IF b THEN c1 ELSE c2)) (ex10 + 1) [(EA_Nop, n20 + (n10 + 1))]
-                           (n20 + (n10 + 1))"
+      have tail: "(to_cfg (IF b THEN c1 ELSE c2)) \<turnstile> (ex10 + 1) \<longrightarrow>\<^bsub>[(EA_Nop, n20 + (n10 + 1))]\<^esub> (n20 + (n10 + 1))"
         using Eif by (auto intro: cfg_path.intros)
       show ?thesis
         using cfg_path_append[OF cfg_path_append[OF head es1_in] tail] H by simp
     next
       assume right: "\<exists>es2. es = (EA_AssumeNot b, en20 + (n10 + 1)) #
                         offset_path (n10 + 1) es2 @ [(EA_Nop, n20 + (n10 + 1))]
-                    \<and> cfg_path (to_cfg c2) en20 es2 ex20"
+                    \<and> (to_cfg c2) \<turnstile> en20 \<longrightarrow>\<^bsub>es2\<^esub> ex20"
       then obtain es2 where H: "es = (EA_AssumeNot b, en20 + (n10 + 1)) #
                         offset_path (n10 + 1) es2 @ [(EA_Nop, n20 + (n10 + 1))]"
-        and p2: "cfg_path (to_cfg c2) en20 es2 ex20"
+        and p2: "(to_cfg c2) \<turnstile> en20 \<longrightarrow>\<^bsub>es2\<^esub> ex20"
         by blast
-      have es2_in: "cfg_path (to_cfg (IF b THEN c1 ELSE c2)) (en20 + (n10 + 1))
-                                   (offset_path (n10 + 1) es2) (ex20 + (n10 + 1))"
+      have es2_in: "(to_cfg (IF b THEN c1 ELSE c2)) \<turnstile> (en20 + (n10 + 1)) \<longrightarrow>\<^bsub>(offset_path (n10 + 1) es2)\<^esub> (ex20 + (n10 + 1))"
         by (rule cfg_path_sub_offset_into[OF c2 p2]) (auto simp: Eif)
-      have head: "cfg_path (to_cfg (IF b THEN c1 ELSE c2)) 0
-                        [(EA_AssumeNot b, en20 + (n10 + 1))] (en20 + (n10 + 1))"
+      have head: "(to_cfg (IF b THEN c1 ELSE c2)) \<turnstile> 0 \<longrightarrow>\<^bsub>[(EA_AssumeNot b, en20 + (n10 + 1))]\<^esub> (en20 + (n10 + 1))"
         using Eif by (auto intro: cfg_path.intros)
-      have tail: "cfg_path (to_cfg (IF b THEN c1 ELSE c2)) (ex20 + (n10 + 1))
-                        [(EA_Nop, n20 + (n10 + 1))] (n20 + (n10 + 1))"
+      have tail: "(to_cfg (IF b THEN c1 ELSE c2)) \<turnstile> (ex20 + (n10 + 1)) \<longrightarrow>\<^bsub>[(EA_Nop, n20 + (n10 + 1))]\<^esub> (n20 + (n10 + 1))"
         using Eif by (auto intro: cfg_path.intros)
       show ?thesis
         using cfg_path_append[OF cfg_path_append[OF head es2_in] tail] H by simp
@@ -1035,13 +1029,13 @@ qed
 lemma cfg_path_While_exit_iff:
   assumes c0: "compile c 0 = (n10, en10, ex10, E10)"
     and c1: "compile c 1 = (n10 + 1, en10 + 1, ex10 + 1, offset_edges 1 E10)"
-  shows "cfg_path (to_cfg (WHILE b DO c)) 0 es (n10 + 1)
+  shows "(to_cfg (WHILE b DO c)) \<turnstile> 0 \<longrightarrow>\<^bsub>es\<^esub> (n10 + 1)
          \<longleftrightarrow>
          (es \<noteq> [] \<and> (\<exists>es_pre. es = es_pre @ [(EA_AssumeNot b, n10 + 1)]
-              \<and> cfg_path (to_cfg (WHILE b DO c)) 0 es_pre 0))"
+              \<and> (to_cfg (WHILE b DO c)) \<turnstile> 0 \<longrightarrow>\<^bsub>es_pre\<^esub> 0))"
 proof (intro iffI)
   (* forward: path to exit \<Longrightarrow> trailing AssumeNot + loop prefix to head *)
-  assume p: "cfg_path (to_cfg (WHILE b DO c)) 0 es (n10 + 1)"
+  assume p: "(to_cfg (WHILE b DO c)) \<turnstile> 0 \<longrightarrow>\<^bsub>es\<^esub> (n10 + 1)"
   have ne: "es \<noteq> []"
   proof (rule ccontr)
     assume "\<not> es \<noteq> []"
@@ -1050,45 +1044,45 @@ proof (intro iffI)
     thus False by simp
   qed
   show "es \<noteq> [] \<and> (\<exists>es_pre. es = es_pre @ [(EA_AssumeNot b, n10 + 1)]
-              \<and> cfg_path (to_cfg (WHILE b DO c)) 0 es_pre 0)"
+              \<and> (to_cfg (WHILE b DO c)) \<turnstile> 0 \<longrightarrow>\<^bsub>es_pre\<^esub> 0)"
   proof (intro conjI)
     show "es \<noteq> []" by (fact ne)
     show "\<exists>es_pre. es = es_pre @ [(EA_AssumeNot b, n10 + 1)]
-              \<and> cfg_path (to_cfg (WHILE b DO c)) 0 es_pre 0"
+              \<and> (to_cfg (WHILE b DO c)) \<turnstile> 0 \<longrightarrow>\<^bsub>es_pre\<^esub> 0"
       using cfg_path_While_split_trailing_exit[OF c0 c1 p ne] by simp
   qed
 next
   (* backward: append loop prefix and final AssumeNot step *)
   assume rhs: "es \<noteq> [] \<and> (\<exists>es_pre. es = es_pre @ [(EA_AssumeNot b, n10 + 1)]
-              \<and> cfg_path (to_cfg (WHILE b DO c)) 0 es_pre 0)"
+              \<and> (to_cfg (WHILE b DO c)) \<turnstile> 0 \<longrightarrow>\<^bsub>es_pre\<^esub> 0)"
   then obtain es_pre where es_eq: "es = es_pre @ [(EA_AssumeNot b, n10 + 1)]"
-    and p0: "cfg_path (to_cfg (WHILE b DO c)) 0 es_pre 0"
+    and p0: "(to_cfg (WHILE b DO c)) \<turnstile> 0 \<longrightarrow>\<^bsub>es_pre\<^esub> 0"
     by auto
   have Ew: "edges (to_cfg (WHILE b DO c)) =
             {(0, EA_Assume b, en10 + 1), (0, EA_AssumeNot b, n10 + 1)}
             \<union> offset_edges 1 E10 \<union> {(ex10 + 1, EA_Nop, 0)}"
     using cfg_edges_entry_exit_While[OF c1] by auto
-  have step: "cfg_path (to_cfg (WHILE b DO c)) 0 [(EA_AssumeNot b, n10 + 1)] (n10 + 1)"
+  have step: "(to_cfg (WHILE b DO c)) \<turnstile> 0 \<longrightarrow>\<^bsub>[(EA_AssumeNot b, n10 + 1)]\<^esub> (n10 + 1)"
     using Ew by (auto intro: cfg_path.intros)
-  show "cfg_path (to_cfg (WHILE b DO c)) 0 es (n10 + 1)"
+  show "(to_cfg (WHILE b DO c)) \<turnstile> 0 \<longrightarrow>\<^bsub>es\<^esub> (n10 + 1)"
     using cfg_path_append[OF p0 step] es_eq by simp
 qed
 
 lemma cfg_path_While_loop_iff:
   assumes c0: "compile c 0 = (n10, en10, ex10, E10)"
     and c1: "compile c 1 = (n10 + 1, en10 + 1, ex10 + 1, offset_edges 1 E10)"
-  shows "cfg_path (to_cfg (WHILE b DO c)) 0 es 0
+  shows "(to_cfg (WHILE b DO c)) \<turnstile> 0 \<longrightarrow>\<^bsub>es\<^esub> 0
          \<longleftrightarrow>
          (es = [] \<or> (\<exists>es_body es_rest.
               es = [(EA_Assume b, en10 + 1)] @ offset_path 1 es_body @ [(EA_Nop, 0)] @ es_rest
-              \<and> cfg_path (to_cfg c) en10 es_body ex10
-              \<and> cfg_path (to_cfg (WHILE b DO c)) 0 es_rest 0))"
+              \<and> (to_cfg c) \<turnstile> en10 \<longrightarrow>\<^bsub>es_body\<^esub> ex10
+              \<and> (to_cfg (WHILE b DO c)) \<turnstile> 0 \<longrightarrow>\<^bsub>es_rest\<^esub> 0))"
 proof (intro iffI)
-  assume p: "cfg_path (to_cfg (WHILE b DO c)) 0 es 0"
+  assume p: "(to_cfg (WHILE b DO c)) \<turnstile> 0 \<longrightarrow>\<^bsub>es\<^esub> 0"
   show "es = [] \<or> (\<exists>es_body es_rest.
               es = [(EA_Assume b, en10 + 1)] @ offset_path 1 es_body @ [(EA_Nop, 0)] @ es_rest
-              \<and> cfg_path (to_cfg c) en10 es_body ex10
-              \<and> cfg_path (to_cfg (WHILE b DO c)) 0 es_rest 0)"
+              \<and> (to_cfg c) \<turnstile> en10 \<longrightarrow>\<^bsub>es_body\<^esub> ex10
+              \<and> (to_cfg (WHILE b DO c)) \<turnstile> 0 \<longrightarrow>\<^bsub>es_rest\<^esub> 0)"
   proof (cases es)
     case Nil
     then show ?thesis by simp
@@ -1101,31 +1095,31 @@ proof (intro iffI)
 next
   assume rhs: "es = [] \<or> (\<exists>es_body es_rest.
               es = [(EA_Assume b, en10 + 1)] @ offset_path 1 es_body @ [(EA_Nop, 0)] @ es_rest
-              \<and> cfg_path (to_cfg c) en10 es_body ex10
-              \<and> cfg_path (to_cfg (WHILE b DO c)) 0 es_rest 0)"
-  from rhs show "cfg_path (to_cfg (WHILE b DO c)) 0 es 0"
+              \<and> (to_cfg c) \<turnstile> en10 \<longrightarrow>\<^bsub>es_body\<^esub> ex10
+              \<and> (to_cfg (WHILE b DO c)) \<turnstile> 0 \<longrightarrow>\<^bsub>es_rest\<^esub> 0)"
+  from rhs show "(to_cfg (WHILE b DO c)) \<turnstile> 0 \<longrightarrow>\<^bsub>es\<^esub> 0"
   proof (elim disjE)
     assume eq: "es = []"
     show ?thesis by (simp add: eq cfg_path.empty)
   next
     assume ex: "\<exists>es_body es_rest.
               es = [(EA_Assume b, en10 + 1)] @ offset_path 1 es_body @ [(EA_Nop, 0)] @ es_rest
-              \<and> cfg_path (to_cfg c) en10 es_body ex10
-              \<and> cfg_path (to_cfg (WHILE b DO c)) 0 es_rest 0"
+              \<and> (to_cfg c) \<turnstile> en10 \<longrightarrow>\<^bsub>es_body\<^esub> ex10
+              \<and> (to_cfg (WHILE b DO c)) \<turnstile> 0 \<longrightarrow>\<^bsub>es_rest\<^esub> 0"
     then obtain es_body es_rest where
         es_eq: "es = [(EA_Assume b, en10 + 1)] @ offset_path 1 es_body @ [(EA_Nop, 0)] @ es_rest"
-      and pb: "cfg_path (to_cfg c) en10 es_body ex10"
-      and pr: "cfg_path (to_cfg (WHILE b DO c)) 0 es_rest 0"
+      and pb: "(to_cfg c) \<turnstile> en10 \<longrightarrow>\<^bsub>es_body\<^esub> ex10"
+      and pr: "(to_cfg (WHILE b DO c)) \<turnstile> 0 \<longrightarrow>\<^bsub>es_rest\<^esub> 0"
       by blast
     have Ew: "edges (to_cfg (WHILE b DO c)) =
               {(0, EA_Assume b, en10 + 1), (0, EA_AssumeNot b, n10 + 1)}
               \<union> offset_edges 1 E10 \<union> {(ex10 + 1, EA_Nop, 0)}"
       using cfg_edges_entry_exit_While[OF c1] by auto
-    have body_in: "cfg_path (to_cfg (WHILE b DO c)) (en10 + 1) (offset_path 1 es_body) (ex10 + 1)"
+    have body_in: "(to_cfg (WHILE b DO c)) \<turnstile> (en10 + 1) \<longrightarrow>\<^bsub>(offset_path 1 es_body)\<^esub> (ex10 + 1)"
       by (rule cfg_path_sub_offset_into[OF c0 pb]) (auto simp: Ew)
-    have head: "cfg_path (to_cfg (WHILE b DO c)) 0 [(EA_Assume b, en10 + 1)] (en10 + 1)"
+    have head: "(to_cfg (WHILE b DO c)) \<turnstile> 0 \<longrightarrow>\<^bsub>[(EA_Assume b, en10 + 1)]\<^esub> (en10 + 1)"
       using Ew by (auto intro: cfg_path.intros)
-    have loopback: "cfg_path (to_cfg (WHILE b DO c)) (ex10 + 1) [(EA_Nop, 0)] 0"
+    have loopback: "(to_cfg (WHILE b DO c)) \<turnstile> (ex10 + 1) \<longrightarrow>\<^bsub>[(EA_Nop, 0)]\<^esub> 0"
       using Ew by (auto intro: cfg_path.intros)
     show ?thesis
       using cfg_path_append[OF cfg_path_append[OF cfg_path_append[OF head body_in] loopback] pr]
