src/Examples/Example_NonTerminating_Safe.thy
@@ -99,8 +99,7 @@ theorem nonterm_safe_at_every_pp:
           (make_rhs_tree (to_cfg nonterm_prog) (ac_tf cfg) (ac_join cfg) (ac_bot cfg) (ac_init cfg))
           (cfg_entry (to_cfg nonterm_prog)))
        (cfg_entry (to_cfg nonterm_prog))"
-  assumes path:     "cfg_path (to_cfg nonterm_prog)
-                              (cfg_entry (to_cfg nonterm_prog)) es v"
+  assumes path:     "(to_cfg nonterm_prog) \<turnstile> (cfg_entry (to_cfg nonterm_prog)) \<longrightarrow>\<^bsub>es\<^esub> v"
   assumes t_in:     "t \<in> edges_collect es {s}"
   shows "t \<in> sound_domain.gamma_state (ac_gamma cfg) (run_analysis cfg nonterm_prog v)"
   by (rule pipeline_sound_path[OF sound join_eq bot_eq tf_sound s_in_gamma
@@ -211,8 +210,7 @@ theorem incr_loop_safe_at_every_pp:
           (make_rhs_tree (to_cfg incr_loop_prog) (ac_tf cfg) (ac_join cfg) (ac_bot cfg) (ac_init cfg))
           (cfg_entry (to_cfg incr_loop_prog)))
        (cfg_entry (to_cfg incr_loop_prog))"
-  assumes path:     "cfg_path (to_cfg incr_loop_prog)
-                              (cfg_entry (to_cfg incr_loop_prog)) es v"
+  assumes path:     "(to_cfg incr_loop_prog) \<turnstile> (cfg_entry (to_cfg incr_loop_prog)) \<longrightarrow>\<^bsub>es\<^esub> v"
   assumes t_in:     "t \<in> edges_collect es {s}"
   shows "t \<in> sound_domain.gamma_state (ac_gamma cfg) (run_analysis cfg incr_loop_prog v)"
   by (rule pipeline_sound_path[OF sound join_eq bot_eq tf_sound s_in_gamma
